Freigen.lean
@@ -1,5 +1,6 @@
 -- This module serves as the root of the `Freigen` library.
 import Freigen.Free
+import Freigen.ITree
 import Freigen.Ast
 import Freigen.Reflect
 import Freigen.Examples
